Splinter/CoordinationLayer/CoordProgramRefinement.i.dfy
@@ -15,14 +15,24 @@ module CoordProgramRefinement {
 
   import Async = CrashTolerantMapSpecMod.async
 
+  // Stitch together a base map, a journal, and the specified ephemeral request state.
+  function IStitch(base: MapAdt, journal: Journal, progress: Async.EphemeralState, syncReqs: SyncReqs) : CrashTolerantMapSpecMod.Variables
+    requires journal.WF()
+    requires journal.CanFollow(base.seqEnd)
+  {
+    // TODO suspicious that 0 is always the stable idx; that can't survive
+    // journal truncation.
+    CrashTolerantMapSpecMod.Variables(journal.VersionsFromBase(base), progress, syncReqs, 0)
+  }
+
   function I(v: CoordProgramMod.Variables) : CrashTolerantMapSpecMod.Variables
   {
     if !Inv(v)
     then CrashTolerantMapSpecMod.InitState()
-    else if MapIsFresh(v)
-      then v.ephemeral.journal.AsCrashTolerantMapSpec(v.persistentSuperblock.mapadt)
-      else v.persistentSuperblock.journal.AsCrashTolerantMapSpec(v.persistentSuperblock.mapadt)
-    
+    else if v.ephemeral.Known?
+      then IStitch(v.persistentSuperblock.mapadt, v.ephemeral.journal, v.ephemeral.progress, v.ephemeral.syncReqs)
+      else IStitch(v.persistentSuperblock.mapadt, v.persistentSuperblock.journal,
+        Async.InitEphemeralState(), map[])
   }
 
   predicate InvLSNTracksPersistentWhenJournalEmpty(v: CoordProgramMod.Variables)
@@ -60,7 +70,7 @@ module CoordProgramRefinement {
     ensures Inv(v)
     ensures I(v) == CrashTolerantMapSpecMod.InitState()
   {
-    assert JournalInterpTypeMod.Mkfs().SyncReqsAt(0) == {}; // trigger set comprehension
+//    assert JournalInterpTypeMod.Mkfs().SyncReqsAt(0) == {}; // trigger set comprehension
   }
 
   lemma InvInductive(v: CoordProgramMod.Variables, v': CoordProgramMod.Variables, uiop: CoordProgramMod.UIOp)
@@ -84,10 +94,16 @@ module CoordProgramRefinement {
       }
 //    case JournalInternalStep(sk) => { assert Inv(v'); }
 //    case SplinterTreeInternalStep(sk) => { assert Inv(v'); }
-      case ReqSyncStep(syncReqId) => {
+      case ReqSyncStep() => {
         assert Inv(v');
       }
-      case CompleteSyncStep(syncReqId) => {
+      case CompleteSyncStep() => {
+        assert Inv(v');
+      }
+      case FreezeJournalStep(newFrozenLSN) => {
+        assert Inv(v');
+      }
+      case FreezeMapAdtStep() => {
         assert Inv(v');
       }
       case CommitStartStep(seqBoundary) => {
@@ -109,41 +125,145 @@ module CoordProgramRefinement {
     var step :| NextStep(v, v', uiop, step);
     match step {
       case LoadEphemeralStateStep() => {
-        assume false;
         assert CrashTolerantMapSpecMod.NextStep(I(v), I(v'),
           CrashTolerantMapSpecMod.NoopOp);
       }
       case RecoverStep(puts) => {
-        assume false;
         assert CrashTolerantMapSpecMod.NextStep(I(v), I(v'),
           CrashTolerantMapSpecMod.NoopOp);
       }
       case QueryStep(key, val) => {
-        assert uiop.OperateOp?;
-        assert uiop.baseOp.ExecuteOp?;
-        assert Query(v, v', uiop, key, val);
-        assert CrashTolerantMapSpecMod.async.DoExecute(
-          Async.Variables(Last(I(v).versions).asyncState, v.ephemeral.journal.reqProgress),
-          Async.Variables(Last(I(v').versions).asyncState, v.ephemeral.journal.reqProgress),
-          uiop.baseOp.req, uiop.baseOp.reply);
-        assert CrashTolerantMapSpecMod.Operate(I(v), I(v'), uiop.baseOp);
         assert CrashTolerantMapSpecMod.NextStep(I(v), I(v'),
           uiop);
-//        assert CrashTolerantMapSpecMod.NextStep(I(v), I(v'),
-//          CrashTolerantMapSpecMod.NoopOp);
       }
       case PutStep() => {
-        assume false;
+//        assert 0<|I(v').versions|;
+        var j := v.ephemeral.journal;
+        var j' := v'.ephemeral.journal;
+        var base := v.persistentSuperblock.mapadt;
+        var base' := v'.persistentSuperblock.mapadt;
+//        var s1 := j'.PruneTail(NextLSN(v)).VersionsFromBase(base');
+//        var s2 := DropLast(j'.VersionsFromBase(base'));
+//        assert |s1| == |s2|;
+
+        // Rob-style SuperTrigger for some sequence rearrangement identity:
+        assert forall i | 0<=i<|DropLast(j'.VersionsFromBase(base'))| ::
+          var seqStart := j'.msgSeq.seqStart;
+          j'.PruneTail(NextLSN(v)).PruneTail(i + seqStart) == j'.PruneTail(i + seqStart);
+
+//        forall i | 0<=i<|s1| ensures s1[i]==s2[i] {
+////          var seqStart := j'.msgSeq.seqStart;
+////          assert seqStart == j'.PruneTail(NextLSN(v)).msgSeq.seqStart;
+////          calc {
+////            j'.PruneTail(NextLSN(v)).PruneTail(i + seqStart);
+////            j'.PruneTail(i + seqStart);
+////          }
+//        }
+//        calc {
+//          v'.ephemeral.journal.PruneTail(NextLSN(v)).VersionsFromBase(v'.persistentSuperblock.mapadt);
+//          DropLast(v'.ephemeral.journal.VersionsFromBase(v'.persistentSuperblock.mapadt));
+//        }
+        assert v.ephemeral.journal == v'.ephemeral.journal.PruneTail(NextLSN(v));
+//        calc {
+//          I(v).versions;
+//          v.ephemeral.journal.VersionsFromBase(v.persistentSuperblock.mapadt);
+//          v.ephemeral.journal.VersionsFromBase(v'.persistentSuperblock.mapadt);
+//            { assert v.ephemeral.journal == v'.ephemeral.journal.PruneTail(NextLSN(v)); }
+//          v'.ephemeral.journal.PruneTail(NextLSN(v)).VersionsFromBase(v'.persistentSuperblock.mapadt);
+//          DropLast(v'.ephemeral.journal.VersionsFromBase(v'.persistentSuperblock.mapadt));
+//          DropLast(I(v').versions);
+//        }
+        var key := uiop.baseOp.req.input.k;
+        var val := uiop.baseOp.req.input.v;
+        var singleton := MsgHistoryMod.Singleton(NextLSN(v), KeyedMessage(key, Define(val)));
+        assert CrashTolerantMapSpecMod.OptionallyAppendVersion(I(v), I(v'));
+
+        assert j.PruneTail(j.msgSeq.seqEnd).msgSeq == j'.PruneTail(j.msgSeq.seqEnd).msgSeq; // seq assembly trigger
+        assert j'.PruneTail(j'.msgSeq.seqEnd) == j'.PruneTail(j.msgSeq.seqEnd).Concat(singleton);  // seq assembly trigger
+        var outerbase := JournalInterpTypeMod.VersionFor(base', j'.PruneTail(j.msgSeq.seqEnd)).asyncState.appv.interp;
+        var outer := outerbase.Put(key, Define(val));
+        var inner := JournalInterpTypeMod.VersionFor(base', j'.PruneTail(j.msgSeq.seqEnd).Concat(singleton)).asyncState.appv.interp;
+
+        assert j'.PruneTail(j.msgSeq.seqEnd).msgSeq.seqEnd == j.msgSeq.seqEnd;
+        assert JournalInterpTypeMod.VersionFor(base', j'.PruneTail(j.msgSeq.seqEnd)).asyncState.appv.interp.seqEnd
+          == j.msgSeq.seqEnd;
+        assert inner.seqEnd
+          == j.msgSeq.seqEnd + 1;
+        assert j'.PruneTail(j.msgSeq.seqEnd).Concat(singleton).msgSeq.seqEnd == j.msgSeq.seqEnd + 1;
+        assert inner.seqEnd == j.msgSeq.seqEnd + 1;
+
+        assert outer.seqEnd == inner.seqEnd;
+
+        forall k
+          ensures outer.mi[k] == inner.mi[k]
+        {
+
+          assert InterpMod.AnyKey(k); // trigger
+          if k == key {
+//            assert outer.mi[k] == Define(val);
+            assert inner == JournalInterpTypeMod.VersionFor(base', j.Concat(singleton)).asyncState.appv.interp;
+            calc {
+              inner.mi[k];
+              j'.PruneTail(j.msgSeq.seqEnd).Concat(singleton).msgSeq.ApplyToInterp(base').mi[k];
+              {
+                var oldMessage := j'.PruneTail(j.msgSeq.seqEnd).Concat(singleton).msgSeq.ApplyToInterpRecursive(base', )
+              }
+              Merge(oldMessage, newMessage);
+            }
+            assert Define(val) == inner.mi[k];
+          } else {
+//            assert outer.mi[k] == outerbase.mi[k];
+            assert outerbase.mi[k] == inner.mi[k];
+          }
+        }
+        calc {
+          JournalInterpTypeMod.VersionFor(base', j'.PruneTail(j.msgSeq.seqEnd)).asyncState.appv.interp.Put(key, Define(val));
+            //here
+          JournalInterpTypeMod.VersionFor(base', j'.PruneTail(j.msgSeq.seqEnd).Concat(singleton)).asyncState.appv.interp;
+          JournalInterpTypeMod.VersionFor(base', j'.PruneTail(j'.msgSeq.seqEnd)).asyncState.appv.interp;
+        }
+        calc {
+          Last(I(v).versions).asyncState.appv.interp.Put(key, Define(val));
+//          Last(j.VersionsFromBase(base)).asyncState.appv.interp.Put(key, Define(val));
+//          JournalInterpTypeMod.VersionFor(base, j.PruneTail(j.msgSeq.seqEnd)).asyncState.appv.interp.Put(key, Define(val));
+//          JournalInterpTypeMod.VersionFor(base, j'.PruneTail(j.msgSeq.seqEnd)).asyncState.appv.interp.Put(key, Define(val));
+//          JournalInterpTypeMod.VersionFor(base', j'.PruneTail(j.msgSeq.seqEnd)).asyncState.appv.interp.Put(key, Define(val));
+//          JournalInterpTypeMod.VersionFor(base', j'.PruneTail(j'.msgSeq.seqEnd)).asyncState.appv.interp;
+//          Last(j'.VersionsFromBase(base')).asyncState.appv.interp;
+          Last(I(v').versions).asyncState.appv.interp;
+        }
+        assert Last(I(v').versions).asyncState.appv.interp == Last(I(v).versions).asyncState.appv.interp.Put(key, Define(val));
+        assert MapSpecMod.Put(
+          Last(I(v).versions).asyncState.appv,
+          Last(I(v').versions).asyncState.appv,
+          key, val);
+
+        assume Async.DoExecute( // TODO darn it
+          Async.Variables(Last(I(v).versions).asyncState, I(v).asyncEphemeral),
+          Async.Variables(Last(I(v').versions).asyncState, I(v').asyncEphemeral),
+          uiop.baseOp.req,
+          uiop.baseOp.reply);
+        assert Async.NextStep(
+          Async.Variables(Last(I(v).versions).asyncState, I(v).asyncEphemeral),
+          Async.Variables(Last(I(v').versions).asyncState, I(v').asyncEphemeral),
+          uiop.baseOp);
+        assert CrashTolerantMapSpecMod.Operate(I(v), I(v'), uiop.baseOp);
         assert CrashTolerantMapSpecMod.NextStep(I(v), I(v'), uiop);
       }
 //    case JournalInternalStep(sk) => { assert Inv(v'); }
 //    case SplinterTreeInternalStep(sk) => { assert Inv(v'); }
-      case ReqSyncStep(syncReqId) => {
+      case ReqSyncStep() => {
         assume false;
         assert CrashTolerantMapSpecMod.NextStep(I(v), I(v'), uiop);
       }
-      case CompleteSyncStep(syncReqId) => {
+      case CompleteSyncStep() => {
         assume false;
+        assert CrashTolerantMapSpecMod.NextStep(I(v), I(v'), uiop);
+      }
+      case FreezeJournalStep(newFrozenLSN) => {
+        assert CrashTolerantMapSpecMod.NextStep(I(v), I(v'), uiop);
+      }
+      case FreezeMapAdtStep() => {
         assert CrashTolerantMapSpecMod.NextStep(I(v), I(v'), uiop);
       }
       case CommitStartStep(seqBoundary) => {
